refactor back simulation interface

omp_compiler/simulation.v
@@ -11,30 +11,55 @@ Section BackSimulation.
   that is "similar" to the new state of the compiled program. *)
   (* NOTE this might not rule out the case where src is terminating but
   tgt is not, but we don't care about this for now *)
-  Class BackSimulation (pass : program -> option program) := {
-    (* Relation on source [s_st] and target [t_st] program states.
-    It seems tricky to define this as an equivalence relation. Since the
-    implicit arguments of Ostate (the global environment and ThreadPool) depend
-    on [genv] the global environment, s_st and t_st have different state types
-    because they can't have the same genv (for instance, their function
-    definitions, which is part of genv, must be different). This makes it
-    difficult to instantiate it as [Equiv (@Ostate _ _)]. *)
-    sim_rel : 
-      forall (sp tp: program) (Hsptp: pass sp = Some tp),
-      @Ostate (Clight.globalenv sp) _ -> @Ostate (Clight.globalenv tp) _ -> Prop;
-    (* a compiler pass is a function from and to Clight programs *)
-    back_simu_proof :
-      forall (sp tp: program)
-      (s : @Ostate (Clight.globalenv sp) _) (t t' : @Ostate (Clight.globalenv tp) _)
-      (* [pass] compiles source program sp to target program tp *)
-      (Hsptp: pass sp = Some tp),
-      (* s_st0, t_st0 are some initial state *)
-      sim_rel sp tp Hsptp s t ->
-      (* t_st0 takes one step to some t_st *)
-      Ostep t t' ->
-      (* then there exists some s_st reachable from s_st0 and s_st≈t_st *)
+
+  
+  (* a compiler pass is a function from and to Clight programs *)
+  Context (pass : program -> option program).
+
+  (* Relation on source [s_st] and target [t_st] program states.
+  It seems tricky to define this as an equivalence relation. Since the
+  implicit arguments of Ostate (the global environment and ThreadPool) depend
+  on [genv] the global environment, s_st and t_st have different state types
+  because they can't have the same genv (for instance, their function
+  definitions, which is part of genv, must be different). This makes it
+  difficult to instantiate it as [Equiv (@Ostate _ _)]. *)
+  Context (rel :
+    forall {sp tp: program},
+    @Ostate (Clight.globalenv sp) _ -> @Ostate (Clight.globalenv tp) _ -> Prop).
+  Arguments rel {sp tp} _ _.
+
+  (* initial state of a program *)
+  Context (init_state : forall (p: program), @Ostate (Clight.globalenv p) _ -> Prop).
+
+  (* probably useful for proving the back simulation property for one step  *)
+  Definition back_simu_one_step (sp tp: program)
+      (s : @Ostate (Clight.globalenv sp) _) (t t' : @Ostate (Clight.globalenv tp) _) (Hsptp: pass sp = Some tp) : Prop :=
+    rel s t ->
+    (* t0 takes one steps to some t' *)
+    Ostep t t' ->
+      (* then there exists some s' reachable from s and s'≈t' *)
       ∃ (s' : @Ostate (Clight.globalenv sp) _),
         Osteps(p:=Build_Prog sp) s s' ∧
-        sim_rel sp tp Hsptp s' t'
-  }.
+        rel s' t'.
+
+  (* Top level refinement theorem. **)
+  Definition back_simu (sp tp: program)
+      (s0 : @Ostate (Clight.globalenv sp) _) (t0 t' : @Ostate (Clight.globalenv tp) _) (Hsptp: pass sp = Some tp) : Prop :=
+    init_state sp s0 ->
+    init_state tp t0 ->
+    (* s0, t0 are some initial state *)
+    rel s0 t0 ->
+    (* t0 takes some steps to some t' *)
+    Osteps(p:=Build_Prog tp) t0 t' ->
+      (* then there exists some s' reachable from s0 and s'≈t' *)
+      ∃ (s' : @Ostate (Clight.globalenv sp) _),
+        Osteps(p:=Build_Prog sp) s0 s' ∧
+        rel s' t'.
+
+  Lemma back_simu_one_step_implies_back_simu:
+    forall sp tp s t t' Hsptp,
+      back_simu_one_step sp tp s t t' Hsptp ->
+      back_simu sp tp s t t' Hsptp.
+  Admitted.
+
 End BackSimulation.
